\documentclass[11pt,a4paper,twoside]{tesis}
% SI NO PENSAS IMPRIMIRLO EN FORMATO LIBRO PODES USAR
% \documentclass[11pt,a4paper]{tesis}

\usepackage{graphicx}
\usepackage[utf8]{inputenc}
\usepackage[english]{babel}
\usepackage[left=3cm,right=3cm,bottom=3.5cm,top=3.5cm]{geometry}
\usepackage{natbib}
\usepackage{mathtools}
\usepackage{ dsfont }
\usepackage{amsthm}

\newtheorem{theorem}{Theorem}[section]
\newtheorem{corollary}{Corollary}[theorem]
\newtheorem{lemma}[theorem]{Lemma}
\newtheorem{proposition}[theorem]{Proposition}
\newtheorem{fact}{Fact}[section]
\theoremstyle{definition}
\newtheorem{definition}{Definition}[section]


\usepackage{amsthm}
 

\DeclarePairedDelimiter{\ceil}{\lceil}{\rceil}
\DeclarePairedDelimiter{\floor}{\lfloor}{\rfloor}


\begin{document}

%%%% CARATULA

\def\autor{Lucas Puterman}
\def\tituloTesis{Números Muy Normales}
\def\runtitulo{Números Muy Normales}
\def\runtitle{Very Normal Numbers}
\def\director{Verónica Becher}
\def\codirector{Olivier Carton}
\def\lugar{Buenos Aires, 2019}
\input{caratula}

%%%% ABSTRACTS, AGRADECIMIENTOS Y DEDICATORIA
\frontmatter
\pagestyle{empty}
\input{abs_esp.tex}

\cleardoublepage
\input{abs_en.tex} % OPCIONAL: comentar si no se quiere

% \cleardoublepage
% \input{agradecimientos.tex} % OPCIONAL: comentar si no se quiere

% \cleardoublepage
% \input{dedicatoria.tex}  % OPCIONAL: comentar si no se quiere

\cleardoublepage
\tableofcontents

\mainmatter
\pagestyle{headings}

%%%% ACA VA EL CONTENIDO DE LA TESIS

\chapter{Introduction}
\section{Normality}
\section{Supernormality}

Let $\lambda > 0$ be a real number.

Let $a_k(\lambda) = \frac{e^{-\lambda}\lambda^k}{k!}$ for $k \geq 0$.

Let $x$ be a sequence over a binary alphabet.

For $u,w$ words, $|w|_u$ is the number of occurrences of $u$ in $w$.

Let $A_{k,n}$ be the frequency of occurrence of words of length $n$ that occur exactly $k$ times in the first $\floor{\lambda(2^n+n-1)}$ symbols of $x$, or what is to say:
$$A_{k,n}(\lambda) = \frac{\#\{w: |w| = n  , |x[1...\lfloor\lambda(2^n+n-1)\rfloor]|_w = k\}}{2^n}$$

\begin{definition}
    $x$ is $\lambda-$supernormal if $$\lim_{n\to\infty} A_{k,n}(\lambda) = a_k(\lambda)$$ for each integer $k \geq 0$.
\end{definition}

\begin{definition}
    $x$ is supernormal if it is $\lambda-$supernormal $\forall \lambda \in \mathds{R}$
\end{definition}

%% ...
\chapter{Supernormality is stronger than normality}
\section{Supernormality implies normality (Proof by Olivier Carton)}



\begin{fact}
    $$\sum_{k \geq 0} a_k(\lambda) = e^{-\lambda}\sum_{k \geq 0} \frac{\lambda^k}{k!} = e^{-\lambda}e^{\lambda} = 1$$
\end{fact}

\begin{fact}
    $$\sum_{k \geq 0} ka_k(\lambda) = e^{-\lambda}\sum_{k \geq 1} \frac{\lambda^k}{(k-1)!} = \lambda e^{-\lambda} \sum_{k \geq 0} \frac{\lambda^k}{k!}= \lambda$$
\end{fact}





\begin{fact}
    $$\sum_{k \geq 0} A_{k,n} = 1$$
\end{fact}

\begin{fact}
    $$A_{k,n} = 0 \textrm{ if } k > \lambda2^n$$
\end{fact}

Let $\epsilon > 0$ be chosen.

Let $k_0$ be chosen such that 
$$\frac{1}{\lambda} \sum_{k > k_0} ka_k(\lambda) < \frac{\epsilon}{2}$$

Let $n_0$ be chosen such that 
$$\forall i,n \: s.t \:  0 \leq i \leq k_0 - 1 \wedge n > n_0 \wedge |A_{i,n}(\lambda) - a_i(\lambda)| \leq \frac{\epsilon\lambda}{2k_0(k_0+1)}$$

$$Rq? = \sum_{i=0}^{k_0-1} ka_k(\lambda) = \lambda - \sum_{k\geq k_0} ka_k(\lambda) \geq (\lambda - \frac{\epsilon}{2})$$

Consider the positions from 1 to $\lfloor\lambda2^n\rfloor$ in $x$. A position is ``blamed'' if the word of length $n$ starting at that position occurs more than $k_0$ times in $x\lfloor\lambda(2^n+n-1)\rfloor$.

The number of non-blamed positions is


\begin{align*}
    \sum_{i=0}^{k-1} iA_{i,n}(\lambda) 2^n &\geq 2^n\sum_{i=0}^{k-1} i (a_i(\lambda) - \frac{\epsilon\lambda}{2k_0(k_0+1)}) \\
    &\geq 2^n \sum_{i=0}^{k-1} ia_{i}(\lambda) - \frac{2^n\epsilon\lambda}{2} \\
    &\geq 2^n\lambda (1-\frac{\epsilon}{2}) - \frac{2^n\epsilon\lambda}{2} \\
    &= 2^n\lambda(1-\epsilon) \\
\end{align*}

We cover the positions of $1\dots \lambda2^n$ by blocks of length such that blocks do not start at a blamed  position. However a block may contain blamed positions.
 
$$\overbracket{\raisebox{6.4pt}{\qquad}}^{n} \overbracket{\raisebox{6.4pt}{\qquad}}^{n}\times\times\overbracket{\;\quad \times}^{n} \times \overbracket{\raisebox{6.4pt}{\qquad}}^{n} \overbracket{\raisebox{6.4pt}{\qquad}}^{n} \times \overbracket{\;\; \times \times}^{n} \times\times\times \overbracket{\raisebox{6.4pt}{\qquad}}^{n}$$


The number of left positions is less than $\epsilon\lambda2^n$. For a fixed word $w$, the number of bad blocks is $o($number of possible blocks$)$. Since each block can occur at most  $k_0 - 1$ times then it is ok.
Hot spot lemma  is needed to conclude.


\section{Normality does not imply supernormality}
We aim to prove that normality does not imply supernormality. For this we prove that the Champernowne sequence, proven to be normal in ~\cite{BC2018}, fails to be supernormal by proving that it is not 1-supernormal.
The strategy followed to achieve this is similar to the ones used in ~\cite{BCC2019} and  ~\cite{PS2019}.


Let $X(n)$ be the concatenation of all words of length $n$ over the alphabet with two simbols $\mathcal{A}=\{0,1\}$ in lexicographic order.  It is clear that $X(n)$ has length $n2^n$. Then, for example:
$$X(2) = 00 \: 01 \: 10 \: 11$$
Note that spaces were added for reading convenience.

Let the Champernowne sequence be the concatenation of $X(n)$ for $n = 1,2,\dots$ Then the first symbols of the Champernowne sequence are:
$$champ = 0 \: 1 \: 00 \: 01 \: 10 \: 11 \: 000 \: 001 \: 010 \: 011 \: 100 \: 101 \: 110 \: 111 \: 0000 \: 0001 \: \dots$$

By the definition of $\lambda$-supernormality, if we take $\lambda = 1$, then we need to prove that

$$\lim_{n\to\infty} A_{k,n}(1) = a_k(1)$$
$$\lim_{n\to\infty} \frac{\#\{w: |w| = n  , |x[1...(2^n+n-1)]|_w = k\}}{2^n} \neq \frac{e^{-1}}{k!}$$

\bigskip

First, let's see that given $d$, we define $k = 2^d$, if we take $n \geq d + k + 1$ then the whole block $X(k)$ covered in the first $2^n$ symbols of Champernowne.


\begin{fact}
    $\forall n, n  \geq 2$ it follows that $\sum_{i=1}^n i2^i < 2^{n + log(n) + 1}$ 
\end{fact}

\begin{fact} \label{p2}
    $X(k)$ accounts for half of the total amount of symbols in the first $2^{d+k+1}$ symbols of Chamernowne.
\end{fact}
\begin{proof}
    $2^{d+k+1} = 2^{d+k}2$ and $X(k)$ has length $k2^k = 2^d2^k = 2^{d+k}$ 
\end{proof}

We prove that Champernowne is not supernormal by showing that the frequence of words of length $k+d+1$ that do not occur in the first $2^{k+d+1}$ symbols of the Champernowne sequence is higher that the expected frequency if it were supernormal.
To accomplish this, we exhaustively look how many different words of length $2^{k+d+1}$ are there within $X(k)$ and give an upper bound for the amount of different words that can appear in the first $2^{k+d+1}$ symbols of the Champernowne sequence.

Now, let's take a look at what the words of length $k + d + 1$ that occur in $X(k)$ look like. There are four different cases that can happen of how a word $x$ is formed with elements from $X(k)$. 
In the following analysis, $u, v$ and $w$ are consecutive words of length $k$ in $X(k)$:

% \begin{itemize}
%   \item \underline{Case 1:} 
%   $$x = u_1 u_2 \dots u_k \quad v_1 v_2 \dots v_{d} v_{d + 1}$$
%     Which means it is the occurrence modulo 0 for a given word $u$ of length $k$ in $X(k)$ plus the remaining $d + 1$ symbols which are taken from the next word.

%   \item \underline{Case 2:} 
%   $$ x = u_{k-d-1} \dots u_k \quad v_1 v_2 \dots v_k$$
%   Which is the case where the word of length $k + d + 1$ is formed from the last $d + 1$ symbols of a word and the whole $k$ symbols of the next word.

%   \item \underline{Case 3:} 
%   $$x = u_{n+1} u_{n+2} \dots u_k \quad  v_1 v_2 \dots v_{d+n+1} $$
% with $n \in \{1,2,\dots ,k - d - 2\}$.

%    Which is the case where the $k + d + 1$ symbols are taken from two words of length $k$ and none of the words is complete.

  
%   \item \underline{Case 4:} 
%   $$ x = u_{k-d-1+n} u_{k-d+n} \dots u_k \quad v_1 v_2 \dots v_k \quad w_1 w_2 \dots w_{d+1-n}$$
%   with $n \in \{1, 2, \dots , d\}$
  
%   Which is the case where the word of length $k + d + 1$ is formed by a full word, and the extra $d + 1$ symbols are taken from both the end of the previous word and the beggining of the next one.

% \end{itemize}



% \subsection{Case Analysis}
% For the simplicity of the proof we define the function $next(w)$ that is used repetidely in the case analysis.

% \begin{definition}
%     Let $next(w):\mathcal{A}^n \rightarrow \mathcal{A}^n $ be $|w|$ times 0 if $w$ only consists of $1s$ and the word that comes after $w$ in lexicographic order in any other case.
% \end{definition}

% \subsubsection{Case 1}
% $$x = u_1 u_2 \dots u_k \quad v_1 v_2 \dots v_{d} v_{d + 1}$$

% This case accounts for the occurrence modulo 0 for a given word u of length $k$ in $X(k)$ plus the remaining $d + 1$ symbols which are taken from the next word.
% As an example, some of the words of length $k + d + 1$ formed from $X(k)$ taking $k = 8, d = 3$ are shown between brackets:

% $$( 00000000 \qquad 0000 ) \; 0001$$
% $$( 00000001 \qquad 0000 ) \; 0010$$
% $$( 00000010 \qquad 0000 ) \; 0011$$
% $$\vdots$$
% $$( 00001110 \qquad 0000 ) \; 1111$$
% $$( 00001111 \qquad 0001 ) \; 0000$$
% $$( 00010000 \qquad 0001 ) \; 0001$$
% $$\vdots$$
% $$( 11111110 \qquad 1111 ) \; 1111$$

% There are two important things to notice here. The first one is that as the words of length $k + d + 1$ are formed by a full word of length $k$ followed by the first $d + 1$ symbols from the next word, in almost every case the first $d + 1$ symbols are equal to the last $d + 1$.
% The only way for this not to happen, is when the last $k - d - 1$ symbols from the first word $u$ are all $1s$, which means that the next word in lexicographic order $v$ consists of $next(v_1 v_2 \dots v_{d + 1})$ concatenated with $next(v_{d + 2} v_{d + 3} \dots v_{k})$.

% The second important thing to notice is that as $X(k)$ is the concatenation of all words of length $k$, all words of length $k$ occur one time in an alligned position modulo $k$. This means that the first $k$ symbols of $x$ takes every possible configuration. 

% These two facts leave two possible schemes for what a word $x$ of case 1 may look like:

% $$\underbrace{\quad A \quad }_{d +1} \qquad \underbrace{\quad B \quad }_{k - d - 1}  \qquad A$$


% $$\underbrace{\quad A \quad }_{d +1} \qquad \underbrace{ 11 \dots 1  }_{k - d - 1}  \qquad next(A) $$

% For the first scheme we have:
% $$2^{d + 1}  (2^{k - d - 1} - 1)$$
% $$ 2\cdot2^{d}  (\frac{2^k}{2\cdot2^d} - 1)$$
% $$ 2^k - \frac{1}{2\cdot2^{d} }$$

% $ 2^k - \frac{1}{2\cdot2^{d} }$ different words.

% For the second scheme we substract one to the cases due to the fact that the last word of length $k$ in $X(k)$ has its continuation outside $X(k)$:
% $$2^{d + 1}   - 1$$
% $$2\cdot 2^d - 1$$
% $ 2\cdot 2^d - 1 $ different words.
% \\

% Counting the whole case together we have $  2^k - \frac{1}{2\cdot2^{d} } + 2\cdot 2^d - 1$ which is less than $2^k -  2\cdot 2^d$ different words.

% \subsubsection{Case 2}
% $$ x = u_{k-d-1} \dots u_k \quad v_1 v_2 \dots v_k$$

% This case accounts for the occurrence modulo 0 for a given word u of length $k$ in $X(k)$ plus the remaining $d + 1$ symbols which are taken from the previous word. This means that in this case the word of length $k + d + 1$ corresponding to the first word of $X(k)$ does not have a corresponding word inside $X(k)$.
% As an example, some of the words of length $k + d + 1$ formed from $X(k)$ taking $k = 8, d = 3$ are shown between brackets:

% $$0000 \; (0000 \qquad 00000001)$$
% $$0000 \; ( \; 0001 \qquad 00000010)$$
% $$\vdots$$
% $$0000 \; (1111 \qquad 10000000)$$
% $$1000 \; (0000 \qquad 10000001)$$
% $$\vdots$$
% $$1111 \; (1110 \qquad 11111111)$$

% As in the previous case, as $X(k)$ is the concatenation of all words of length $k$, all words of length $k$ occur one time in an alligned position modulo $k$. This means that the last $k$ symbols of $x$ take every possible configuration.
% The other important thing to notice is that as the first $d + 1$ symbols of $x$ come from the word $u$ which occups exactly before $v$ in lexicographic order, then: 
% $$next(u_{k-d-1} u_{k-d} \dots u_k) = u_{v-d-1} v_{k-d} \dots v_k$$

% This leaves only one possible scheme for what a word $x$ of case 2 may look like:

% $$\underbrace{\quad A \quad }_{d +1} \qquad \underbrace{\quad B \quad }_{k - d - 1}  \qquad next(A)$$

% This scheme gives us the following amount of different words that may occur:
% $$(2^{d + 1} 2^{k-d})-1$$
% $$ 2\cdot 2^d  (\frac{2^k}{2^d}) - 1$$
% $$ 2 \cdot 2^k - 1$$

% $ 2 \cdot 2^k - 1 $ different words which is less than $2 \cdot 2^k$ diffrent words.

% \subsubsection{Case 3}
% $$x = u_{n+1} u_{n+2} \dots u_k \quad  v_1 v_2 \dots v_{d+n+1} $$
% with $n \in \{1,2,\dots ,k - d - 2\}$.
% \\

% This case accounts for when the $k + d + 1$ symbols are taken from two words of length $k$ and none of the words is complete.
% As an example, some of the words of length $k + d + 1$ formed from $X(k)$ taking $k = 8, d = 3$ are shown between brackets
% Some extra spaces are added within $u$ and $v$ to make clear the scheme explained later.
% Taking $n = 1$.

% $$0\; (0000\; 000 \qquad 0 \;0000 ) \;001$$
% $$0\; (0000 \;001 \qquad 0 \;0000 ) \;010$$
% $$\vdots$$
% $$0\; (0001 \;110 \qquad 0 \;0001 ) \;111$$
% $$0\; (0001 \;111 \qquad 0 \;0010 ) \;000$$
% $$0\; (0010 \;000 \qquad 0 \;0010 ) \;001$$
% $$\vdots$$
% $$1\; (1111 \;101 \qquad 1 \;1111 ) \;110$$
% $$0\; (1111 \;110 \qquad 1 \;1111 ) \;111$$

% Taking $n = k - d - 2 = 3$

% $$000\; (0000\; 0 \qquad 000 \;0000 ) \;1$$
% $$000\; (0000\; 1 \qquad 000 \;0001 ) \;0$$
% $$000\; (0001\; 0 \qquad 000 \;0001 ) \;1$$
% $$000\; (0001\; 1 \qquad 000 \;0010 ) \;0$$
% $$\vdots$$
% $$111\; (1110\; 1 \qquad 111 \;1111 ) \;0$$
% $$111\; (1111\; 0 \qquad 111 \;1111 ) \;1$$

% In this case, it also happens that as $X(k)$ is the concatenation of all words of length $k$, for each value of $n$, all words of length $k$ take the $u$ position once, except the last of the words of length $k$ in $X(k)$.

% It is important to notice that for a given value of $n$, the first $n$ symbols of $u$ are not be considered to form $x$. This means that it can be interepreted that the symbols from  $u$ that are considered are, the first $d + 1$ symbols after $n$ which are called $A$ and the remaining $k - d - 1 - n$ symbols which are be called $B$.

% Now, if we divide the $n + d + 1$ symbols that are used from $v$ to form $x$ into the first $n$ symbols which are called $C$ and the remaining $d + 1$ symbols, it is possible to see that these $d + 1$ symbols are always equal to the symbols from $A$ except for the case where $B$ = $11\dots1$ as they account for the same indexes of $u$ and $v$ and $v$ comes immediately after $u$ in lexicographic order. 


% These leave two possible schemes for what a word x of case 3 may look like:

% $$\underbrace{\quad A \quad }_{d +1} \qquad \underbrace{\quad B \quad }_{k - d - 1 - n}  \qquad \underbrace{\quad C \quad }_{n} \qquad A$$

% $$\underbrace{\quad A \quad }_{d +1} \qquad \underbrace{\; 11\dots1 \; }_{k - d - 1 - n}  \qquad \underbrace{\quad C \quad }_{n} \qquad next(A)$$

% Looking closely at the first scheme, it is possible to see, if we put together $B$ and $C$ which have length $k - d - 1 - n$ and $n$ respectively, that we have the following scheme:

% $$\underbrace{\quad A \quad }_{d +1} \qquad \underbrace{\quad B \quad }_{k - d - 1}  \qquad A$$

% which is exactly the same one as in case 1. This means that all the possible words that can be formed following this scheme don't yield any new words.
% \\
% The same thing happens with the second scheme when concatenating $11\dots1$ with $C$:

% $$\underbrace{\quad A \quad }_{d +1} \qquad \underbrace{\; 11\dots1C \; }_{k - d - 1}  \qquad next(A)$$

% Which is a particular case of case 2.

% This means that for case 3 there are no words that appear that should be taken into account as new words.


% \subsubsection{Case 4}
% $$ x = u_{k-d-1+n} u_{k-d+n} \dots u_k \quad v_1 v_2 \dots v_k \quad w_1 w_2 \dots w_{d+1-n}$$
% with $n \in \{1, 2, \dots , d\}$

% This case accounts for when the $k + d + 1$ symbols are taken from three words of length $k$. The $k$ symbols of $v$ are used and the remaining $d + 1$ symbols are taken from both the previous and the following words $u$ and $w$.
% As an example, some of the words of length $k + d + 1$ formed from $X(k)$ taking $k = 8, d = 3$ are shown between brackets
% Some extra spaces are added within $u$ and $v$ to make clear the scheme that is explained later.

% Taking $n = 1$.
% $$0000000\; (0 \qquad 000 \; 0000 \; 1 \qquad 000) \: 00010$$
% $$0000000\; (1 \qquad 000 \; 0001 \; 0 \qquad 000) \: 00011$$
% $$\vdots$$
% $$0011111\; (0 \qquad 001 \; 1111 \; 1 \qquad 001) \: 10000$$
% $$0011111\; (1 \qquad 010 \; 0000 \; 0 \qquad 010) \: 00001$$
% $$\vdots$$
% $$1111110\; (1 \qquad 111 \; 1111 \; 0 \qquad 111) \: 11111$$

% Taking $n = 2$.
% $$000000\; (00 \qquad 00 \; 0000 \; 01 \qquad 00) \: 000010$$
% $$000000\; (01 \qquad 00 \; 0000 \; 10 \qquad 00) \: 000011$$
% $$\vdots$$
% $$001111\; (01 \qquad 00 \; 1111 \; 10 \qquad 00) \: 111111$$
% $$001111\; (10 \qquad 00 \; 1111 \; 11 \qquad 01) \: 000000$$
% $$001111\; (11 \qquad 01 \; 0000 \; 00 \qquad 01) \: 000001$$
% $$\vdots$$
% $$111111\; (01 \qquad 11 \; 1111 \; 10 \qquad 11) \: 111111$$

% In this case, it also happens that as $X(k)$ is the concatenation of all words of length $k$, for each value of $n$, 
% all words of length $k$ take the $u$ position once, except the last of the words of length $k$ in $X(k)$.

% We call $A$ the first $n$ symbols of $x$ which are taken from the end of $v$. The following $d + 1 - n$ symbols which are the first of $v$ are called $B$ and it happens that unless the remaining symbols of $v$ are all $1s$, 
% they are be the same as the last $d + 1 - n$ of $x$ because these symbols are the first $d + 1 - n$ from $w$.
% Now, we consider the remaining $k - d - 1 + n$ symbols from $v$ as two blocks, one block $C$ of length $k - d - 1$ and the remaining $n$ symbols which are exctly $next(A)$ as $v$ is the next word in lexicographic order after $u$.
% This yields the two following schemes:

% $$\underbrace{\quad A \quad }_{n} \qquad \underbrace{\quad B \quad }_{d + 1 - n}  \qquad \underbrace{\quad C \quad }_{k-d+1} \qquad next(A) \qquad B$$

% $$\underbrace{\quad 11\dots10 \quad }_{n} \qquad \underbrace{\quad B \quad }_{d + 1 - n}  \qquad \underbrace{\; 11\dots1 \; }_{k-d+1} \qquad next(A) \qquad next(B)$$

% For the first scheme we have:

% $$\sum_{n=1}^{d}(2^n - 1) (2^{d + 1 - n}) (2^{k - d - 1})$$
% $$\sum_{n=1}^{d}(2^n - 1) (\frac{2 \cdot 2^d}{2^n})     (\frac{2^k}{2 \cdot 2^d})$$
% $$ 2^k \sum_{n=1}^{d} \frac{2^n - 1}{2^n} $$

% % Here we would need to substract the cases for when $v$ is the last word of $X(k)$, however as we are giving an upper bound for the words that appear in Champernowne, the result still holds taking this number.

% For the second scheme we have:

% $$ \sum_{n=1}^{d} 2^{d + 1 - n}$$
% $$ \sum_{n=1}^{d} 2 \frac{2^d}{2^{- n}}$$
% $$ 2 \cdot 2^d \sum_{n=1}^{d} 2^{- n}$$

% When putting them both together we get:

% $$  2^k \sum_{n=1}^{d} \frac{2^n - 1}{2^n}  + 2 \cdot 2^d \sum_{n=1}^{d} 2^{- n} < d2^k + 2 \cdot 2^d$$

% \subsubsection{Special Cases}

% We consider the last to words of $X(k)$ as special cases. The last word of $X(k)$ does not apply to any of the cases since there are no words $v$ and $w$ inside $X(k)$ to consider the cases. Something similar occurs with the word previous to the last one and case 4. 
% While it is true that we do know which words come immediately after  $X(k)$, which are the first words of size $d+k+2$ in lexicographic order, as we are giving an upper bound, it is valid to consider all of these as different words to all of the ones considered in the previous cases.
% By doing this, we would have to consider $d+k+1$ new words for the last word and $d$ words for the previous one. So this yields $2d+k+1$ words to consider.


\subsection{Bounding words that appear in Champernowne}

If the Champernowne sequence were supernormal then the expected frequency of words that appear at least one time in the first $2^n + n -1$ symbols would be:
$$\lim_{n\to\infty} \frac{\#\{w: |w| = n  , |champ[1...(2^n+n-1)]|_w > 0\}}{2^n}  = 1 - e^{-1}$$


Now, by Fact \ref{p2} we know that $X(k)$ accounts for half of the words of the first $2^{d+k+1}$ symbols of Champernowne. 
If we analize what happens with words of length $d+k+1$ using the bounds we have for the occurrences of different words within $X(k)$ and we assume that the remaining $2^{d+k} + d + k - 1$  symbols are all different, then



$$\lim_{d\to\infty} \frac{\#\{w : |w| = d+k+1, |champ[1 \dots 2^{d+k+1}+d+k+1-1]|_w > 0 \}}{2^{d+k+1}} =$$
$$\lim_{d\to\infty} \frac{\#\{w : |w| = d+k+1, |champ[1 \dots 2^{d+k+1}+d+k]|_w > 0 \}}{2^{d+k+1}} <$$
$$\lim_{d\to\infty} \frac{ \textrm{case 1} + \textrm{case 2}+ \textrm{case 4} + \textrm{last 2} + \textrm{other half} + (d + k) }{2^{d+k+1}} =$$
$$\lim_{d\to\infty} \frac{(2^k - 2\cdot 2^d) + (2 \cdot 2^k)+ (d2^k + 2 \cdot 2^d) + (2d+k+1) + (2^{d+k}) + (d + k) }{2^{d+k+1}} =$$
$$\lim_{d\to\infty} \frac{(2^k - 2k) + (2 \cdot 2^k)+ (d2^k + 2k) + (3d+2k+1) + (k2^{k})}{2k2^{k}} =$$
$$\lim_{d\to\infty} \frac{3\cdot2^k + d2^k  + 3d+2k+1}{2k2^{k}} + \frac{1}{2} =$$
$$\lim_{d\to\infty} \frac{3}{2k} + \frac{d}{2k} + \frac{d}{k2^{k}} + \frac{1}{2\cdot2^{k}} + \frac{1}{2k2^{k}} + \frac{1}{2} = \frac{1}{2} < 1 - e^{-1}$$


Finally, if in the original sequence we consider that the $n$'s such thar $n = d + 2^d + 1$ are a subsequence of $n=1,2,\dots$ then we can say that if
$$\lim_{n\to\infty} \frac{\#\{w: |w| = n  , |champ[1...(2^n+n-1)]|_w = k\}}{2^n}$$
exists, then it is not $1 - e^{-1}$.
This implies that Champernowne is not 1-supernormal which means it is not supernormal.

\begin{corollary}
If $x$ is a normal number it is not implied that $x$ is supernormal.
\end{corollary}


% \chapter{Conclusions and Further Work}

%%%% BIBLIOGRAFIA
\chapter{Bibliography}
\backmatter
\bibliographystyle{alpha}
\bibliography{tesis}



\end{document}
